Com.v
@@ -6,10 +6,12 @@ Import BexpNotations.
 From Rela Require Import Proc.
 From Rela Require Import Sigma.
 From Coq Require Import Lia.
+From Coq Require Import Lists.List.
+Import ListNotations.
 
 (** Definition of assertion **)
 
-Definition assertion : Type := sigma -> Prop.
+Definition assertion : Type := list sigma -> Prop.
 
 (** Defintion of command and program **)
 
@@ -44,7 +46,6 @@ Inductive ceval : com -> sigma -> Psi.psi -> sigma -> Prop :=
     aeval s a = n ->
     ceval (CAssr x a) s ps ((s x) !-> n ; s)
   | E_Assert: forall s ps (b : assertion),
-    b s ->
     ceval (CAssert b) s ps s
   | E_IfTrue : forall s s' ps b p1 p2,
       beval s b = true ->
@@ -77,7 +78,7 @@ Lemma ceval_inf_loop s ps s' :
 ceval (CWhile BTrue CSkip (fun _ => True)) s ps s' -> False.
 Proof.
   intros Heval.
-  remember (CWhile BTrue CSkip (fun _ : Sigma.sigma => True)) as original_command eqn:Horig.
+  remember (CWhile BTrue CSkip (fun _ : list Sigma.sigma => True)) as original_command eqn:Horig.
   induction Heval;try inversion Horig.
   * inversion Horig;subst. inversion H.
   * inversion Horig;subst.
